wip: start proving bignumQ

code/experimental/ed25519/Hacl.Spec.BignumQ.Mul.fst
@@ -3,6 +3,8 @@ module Hacl.Spec.BignumQ.Mul
 open FStar.Mul
 open Lib.IntTypes
 
+module S = Spec.Ed25519
+
 #reset-options "--z3rlimit 50 --max_fuel 0 --max_ifuel 0"
 
 let qelem5 = (uint64 & uint64 & uint64 & uint64 & uint64)
@@ -10,46 +12,263 @@ let qelem_wide5 = (uint64 & uint64 & uint64 & uint64 & uint64 & uint64 & uint64 
 let qelem_after_mul5 = (uint128 & uint128 & uint128 & uint128 & uint128 & uint128 & uint128 & uint128 & uint128)
 
 
+let scale64 = s:nat{s <= 256}
+let nat5 = (nat & nat & nat & nat & nat)
+
+let scale64_5 = x:nat5{let (x1,x2,x3,x4,x5) = x in
+		       x1 <= 256 /\ x2 <= 256 /\ x3 <= 256 /\ x4 <= 256 /\ x5 <= 256}
+
+abstract
+let pow56: (pow56: pos { pow2 64 == 256 * pow56 /\ pow2 128 == 65536 * pow56 * pow56 /\ pow56 == pow2 56 }) =
+  let pow56: pos = normalize_term (pow2 56) in
+  assert_norm (pow56 > 0);
+  assert_norm (pow56 == pow2 56);
+  assert_norm (pow2 64 == 256 * pow56);
+  assert_norm (pow2 128 == 65536 * pow56 * pow56);
+  pow56
+
+abstract
+let pow112: (pow112: pos { pow112 == pow2 112 /\ pow112 == pow56 * pow56}) =
+  let pow112: pos = normalize_term (pow2 112) in
+  assert_norm (pow112 > 0);
+  assert_norm (pow112 == pow2 112);
+  assert_norm (pow2 112 == pow2 56 * pow2 56);
+  pow112
+
+abstract
+let pow168: (pow168: pos { pow168 == pow2 168 /\ pow168 == pow56 * pow56 * pow56}) =
+  let pow168: pos = normalize_term (pow2 168) in
+  assert_norm (pow168 > 0);
+  assert_norm (pow168 == pow2 168);
+  assert_norm (pow2 168 == pow2 56 * pow2 56 * pow2 56);
+  pow168
+
+abstract
+let pow224: (pow224: pos { pow224 == pow2 224 /\ pow224 == pow56 * pow56 * pow56 * pow56}) =
+  let pow224: pos = normalize_term (pow2 224) in
+  assert_norm (pow224 > 0);
+  assert_norm (pow224 == pow2 224);
+  assert_norm (pow2 224 == pow2 56 * pow2 56 * pow2 56 * pow2 56);
+  pow224
+
+
 inline_for_extraction noextract
-val make_m: unit -> m:qelem5
+let max56 = pow56 - 1
+
+let qelem_fits1 (x:uint64) (m:scale64) =
+  uint_v x <= m * max56
+
+let qelem_fits5 (f:qelem5) (m:scale64_5) =
+  let (x1,x2,x3,x4,x5) = f in
+  let (m1,m2,m3,m4,m5) = m in
+  qelem_fits1 x1 m1 /\
+  qelem_fits1 x2 m2 /\
+  qelem_fits1 x3 m3 /\
+  qelem_fits1 x4 m4 /\
+  qelem_fits1 x5 m5
+
+
+noextract
+val as_nat5: f:qelem5 -> GTot nat
+let as_nat5 f =
+  let (s0, s1, s2, s3, s4) = f in
+  v s0 + v s1 * pow56 + v s2 * pow112 + v s3 * pow168 + v s4 * pow224
+
+
+inline_for_extraction noextract
+let mask56 : x:uint64{v x == pow2 56 - 1} =
+  assert_norm (pow2 56 - 1 == 0xffffffffffffff);
+  u64 0xffffffffffffff
+
+
+inline_for_extraction noextract
+let mask40 : x:uint64{v x == pow2 40 - 1} =
+  assert_norm (pow2 40 - 1 == 0xffffffffff);
+  u64 0xffffffffff
+
+
+inline_for_extraction noextract
+val make_m: unit -> m:qelem5{qelem_fits5 m (1, 1, 1, 1, 1) /\ as_nat5 m == S.q}
 let make_m () =
   let m0 = u64 0x12631a5cf5d3ed in
   let m1 = u64 0xf9dea2f79cd658 in
   let m2 = u64 0x000000000014de in
   let m3 = u64 0x00000000000000 in
   let m4 = u64 0x00000010000000 in
+  assert_norm (as_nat5 (m0, m1, m2, m3, m4) == S.q);
   (m0, m1, m2, m3, m4)
 
 
 inline_for_extraction noextract
-val make_mu: unit -> m:qelem5
+val make_mu: unit -> m:qelem5{qelem_fits5 m (1, 1, 1, 1, 1) /\ as_nat5 m == pow2 512 / S.q}
 let make_mu m =
   let m0 = u64 0x9ce5a30a2c131b in
   let m1 = u64 0x215d086329a7ed in
   let m2 = u64 0xffffffffeb2106 in
   let m3 = u64 0xffffffffffffff in
   let m4 = u64 0x00000fffffffff in
+  assert_norm (as_nat5 (m0, m1, m2, m3, m4) == pow2 512 / S.q);
   (m0, m1, m2, m3, m4)
 
 
+val lemma_choose_step:
+    bit:uint64{v bit <= 1}
+  -> x:uint64
+  -> y:uint64
+  -> Lemma
+     (let mask = bit -. u64 1 in
+      let z = x ^. (mask &. (x ^. y)) in
+      if v bit = 1 then z == x else z == y)
+
+let lemma_choose_step bit p1 p2 =
+  let mask = bit -. u64 1 in
+  assert (v bit == 0 ==> v mask == pow2 64 - 1);
+  assert (v bit == 1 ==> v mask == 0);
+  let dummy = mask &. (p1 ^. p2) in
+  logand_lemma mask (p1 ^. p2);
+  assert (v bit == 1 ==> v dummy == 0);
+  assert (v bit == 0 ==> v dummy ==  v (p1 ^. p2));
+  let p1' = p1 ^. dummy in
+  assert (v dummy == v (if v bit = 1 then u64 0 else (p1 ^. p2)));
+  logxor_lemma p1 p2
+
+
 inline_for_extraction noextract
-val choose: b:uint64{v b == 0 \/ v b == 1} -> x:qelem5 -> y:qelem5 -> z:qelem5
+val choose:
+    b:uint64
+  -> x:qelem5
+  -> y:qelem5 ->
+  Pure qelem5
+  (requires v b == 0 \/ v b == 1)
+  (ensures fun z -> if v b = 1 then z == x else z == y)
+
 let choose b (x0, x1, x2, x3, x4) (y0, y1, y2, y3, y4) =
   let mask = b -. u64 1 in
-  let z0 = ((y0 ^. x0) &. mask) ^. x0 in
-  let z1 = ((y1 ^. x1) &. mask) ^. x1 in
-  let z2 = ((y2 ^. x2) &. mask) ^. x2 in
-  let z3 = ((y3 ^. x3) &. mask) ^. x3 in
-  let z4 = ((y4 ^. x4) &. mask) ^. x4 in
+  let z0 = x0 ^. (mask &. (x0 ^. y0)) in
+  lemma_choose_step b x0 y0;
+  let z1 = x1 ^. (mask &. (x1 ^. y1)) in
+  lemma_choose_step b x1 y1;
+  let z2 = x2 ^. (mask &. (x2 ^. y2)) in
+  lemma_choose_step b x2 y2;
+  let z3 = x3 ^. (mask &. (x3 ^. y3)) in
+  lemma_choose_step b x3 y3;
+  let z4 = x4 ^. (mask &. (x4 ^. y4)) in
+  lemma_choose_step b x4 y4;
   (z0, z1, z2, z3, z4)
 
 
 inline_for_extraction noextract
-val subm_step: x:uint64 -> y:uint64 -> uint64 & uint64
+val subm_step: x:uint64 -> y:uint64 ->
+  Pure (uint64 & uint64)
+  (requires v x < pow56 /\ v y <= pow56)
+  (ensures fun (b, t) ->
+    v b <= 1 /\ qelem_fits1 t 1 /\
+    v x - v y == v t - v b * pow56)
+
 let subm_step x y =
   let b = (x -. y) >>. 63ul in
-  let t = (b <<. 56ul) +. x -. y in
+  //assert (if v x >= v y then v b == 0 else v b == 1);
+  let lshift56 = (b <<. 56ul) in
+  //assert (if v x >= v y then v lshift56 == 0 else v lshift56 == pow56);
+  //assert (v lshift56 == v b * pow56);
+  //assert (v ((b <<. 56ul) +! x) == v b * pow56 + v x);
+  let t = ((b <<. 56ul) +! x) -! y in
   b, t
+
+
+inline_for_extraction noextract
+val subm_conditional: x:qelem5 ->
+  Pure qelem5
+  (requires
+    qelem_fits5 x (1, 1, 1, 1, 1))
+  (ensures fun r ->
+    qelem_fits5 r (1, 1, 1, 1, 1) /\
+    (if as_nat5 x >= S.q then as_nat5 r == as_nat5 x - S.q else as_nat5 r == as_nat5 x))
+
+let subm_conditional (x0, x1, x2, x3, x4) =
+  let (y0, y1, y2, y3, y4) = make_m () in
+  let (b0, t0) = subm_step x0 y0 in
+  assert (v x0 - v y0 == v t0 - v b0 * pow56);
+  let (b1, t1) = subm_step x1 (y1 +! b0) in
+  assert (v x1 - v y1 - v b0 == v t1 - v b1 * pow56);
+  let (b2, t2) = subm_step x2 (y2 +! b1) in
+  assert (v x2 - v y2 - v b1 == v t2 - v b2 * pow56);
+  let (b3, t3) = subm_step x3 (y3 +! b2) in
+  assert (v x3 - v y3 - v b2 == v t3 - v b3 * pow56);
+  let (b4, t4) = subm_step x4 (y4 +! b3) in
+  assert (v x4 - v y4 - v b3 == v t4 - v b4 * pow56);
+
+  assert (
+    as_nat5 (t0, t1, t2, t3, t4) - v b4 * pow56 * pow224 ==
+    as_nat5 (x0, x1, x2, x3, x4) - as_nat5 (y0, y1, y2, y3, y4));
+
+  assert_norm (pow56 * pow224 = pow2 280);
+  assert (as_nat5 (t0, t1, t2, t3, t4) - v b4 * pow2 280 == as_nat5 (x0, x1, x2, x3, x4) - S.q);
+  //assert (as_nat5 (x0, x1, x2, x3, x4) < pow2 280);
+  //assert (if v b4 = 0 then as_nat5 (x0, x1, x2, x3, x4) >= S.q else as_nat5 (x0, x1, x2, x3, x4) < S.q);
+  assert (if as_nat5 (x0, x1, x2, x3, x4) >= S.q then v b4 == 0 else v b4 == 1);
+  //assert (qelem_fits5 (t0, t1, t2, t3, t4) (1, 1, 1, 1, 1));
+  let (z0, z1, z2, z3, z4) = choose b4 (x0, x1, x2, x3, x4) (t0, t1, t2, t3, t4) in
+  assert (
+    if as_nat5 (x0, x1, x2, x3, x4) >= S.q
+    then as_nat5 (z0, z1, z2, z3, z4) == as_nat5 (t0, t1, t2, t3, t4)
+    else as_nat5 (z0, z1, z2, z3, z4) == as_nat5 (x0, x1, x2, x3, x4));
+  assert (
+    if as_nat5 (x0, x1, x2, x3, x4) >= S.q
+    then v b4 == 0 /\ as_nat5 (z0, z1, z2, z3, z4) == as_nat5 (t0, t1, t2, t3, t4)
+    else v b4 == 1 /\ as_nat5 (z0, z1, z2, z3, z4) == as_nat5 (x0, x1, x2, x3, x4));
+  (z0, z1, z2, z3, z4)
+
+
+inline_for_extraction noextract
+val carry56: x:uint64 ->
+  Pure (uint64 & uint64)
+  (requires v x <= pow2 57)
+  (ensures  fun (t, c) ->
+    v t < pow56 /\ v c <= 2 /\
+    v x == v c * pow56 + v t)
+
+let carry56 x =
+  let carry = x >>. 56ul in
+  FStar.Math.Lemmas.pow2_minus 57 56;
+  let t     = x &. mask56 in
+  assert_norm (pow2 56 < pow2 64);
+  mod_mask_lemma x 56ul;
+  assert (v (mod_mask #U64 #SEC 56ul) == v mask56);
+  assert (v t == v x % pow2 56);
+  assert (v x == v carry * pow2 56 + v t);
+  t, carry
+
+
+inline_for_extraction noextract
+val add_modq5:
+    x:qelem5
+  -> y:qelem5
+  -> Pure qelem5
+    (requires
+      qelem_fits5 x (1, 1, 1, 1, 1) /\
+      qelem_fits5 y (1, 1, 1, 1, 1) /\
+      as_nat5 x < S.q /\ as_nat5 y < S.q)
+    (ensures fun z ->
+      qelem_fits5 z (1, 1, 1, 1, 1) /\
+      as_nat5 z % S.q == (as_nat5 x + as_nat5 y) % S.q)
+
+let add_modq5 (x0, x1, x2, x3, x4) (y0, y1, y2, y3, y4) =
+  assert_norm (pow56 - 1 + pow56 - 1 == pow2 57 - 2);
+  let (t0, c0) = carry56 (x0 +! y0) in
+  let (t1, c1) = carry56 (x1 +! y1 +! c0) in
+  let (t2, c2) = carry56 (x2 +! y2 +! c1) in
+  let (t3, c3) = carry56 (x3 +! y3 +! c2) in
+  let t4 = x4 +! y4 +! c3 in
+  assert (as_nat5 (t0, t1, t2, t3, t4) == as_nat5 (x0, x1, x2, x3, x4) + as_nat5 (y0, y1, y2, y3, y4));
+  let (o0, o1, o2, o3, o4) = subm_conditional (t0, t1, t2, t3, t4) in
+  assert (
+    if as_nat5 (t0, t1, t2, t3, t4) >= S.q
+    then (
+      FStar.Math.Lemmas.sub_div_mod_1 (as_nat5 (t0, t1, t2, t3, t4)) S.q;
+      as_nat5 (o0, o1, o2, o3, o4) % S.q == as_nat5 (t0, t1, t2, t3, t4) % S.q)
+    else as_nat5 (o0, o1, o2, o3, o4) == as_nat5 (t0, t1, t2, t3, t4));
+  (o0, o1, o2, o3, o4)
 
 
 inline_for_extraction noextract
@@ -72,31 +291,10 @@ let sub_mod_264 (x0, x1, x2, x3, x4) (y0, y1, y2, y3, y4) =
 
 
 inline_for_extraction noextract
-val subm_conditional: x:qelem5 -> z:qelem5
-let subm_conditional (x0, x1, x2, x3, x4) =
-  let (y0, y1, y2, y3, y4) = make_m () in
-  let (b, t0) = subm_step x0 y0 in
-  let (b, t1) = subm_step x1 (y1 +. b) in
-  let (b, t2) = subm_step x2 (y2 +. b) in
-  let (b, t3) = subm_step x3 (y3 +. b) in
-  let (b, t4) = subm_step x4 (y4 +. b) in
-  let (z0, z1, z2, z3, z4) = choose b (x0, x1, x2, x3, x4) (t0, t1, t2, t3, t4) in
-  (z0, z1, z2, z3, z4)
-
-
-inline_for_extraction noextract
-val carry56: x:uint64 -> uint64 & uint64
-let carry56 x =
-  let carry = x >>. 56ul in
-  let t     = to_u64 x &. u64 0xffffffffffffff in
-  carry, t
-
-
-inline_for_extraction noextract
 val carry56_wide: x:uint128 -> uint128 & uint64
 let carry56_wide x =
   let carry = x >>. 56ul in
-  let t     = to_u64 x &. u64 0xffffffffffffff in
+  let t     = to_u64 x &. mask56 in
   carry, t
 
 
@@ -124,7 +322,7 @@ let low_mul_5 (x0, x1, x2, x3, x4) (y0, y1, y2, y3, y4) =
   let (carry, t1) = carry56_wide (xy01 +. xy10 +. carry) in
   let (carry, t2) = carry56_wide (xy02 +. xy11 +. xy20 +. carry) in
   let (carry, t3) = carry56_wide (xy03 +. xy12 +. xy21 +. xy30 +. carry) in
-  let t4 = to_u64 (xy04 +. xy13 +. xy22 +. xy31 +. xy40 +. carry) &. u64 0xffffffffff in //mod40
+  let t4 = to_u64 (xy04 +. xy13 +. xy22 +. xy31 +. xy40 +. carry) &. mask40 in
   (t0, t1, t2, t3, t4)
 
 
@@ -183,6 +381,7 @@ let carry (z0, z1, z2, z3, z4, z5, z6, z7, z8) =
   let x9 = to_u64 carry in
   (x0, x1, x2, x3, x4, x5, x6, x7, x8, x9)
 
+
 inline_for_extraction noextract
 val mul_carry5: qelem5 -> qelem5 -> qelem_wide5
 let mul_carry5 (x0, x1, x2, x3, x4) (y0, y1, y2, y3, y4) =
@@ -194,7 +393,7 @@ let mul_carry5 (x0, x1, x2, x3, x4) (y0, y1, y2, y3, y4) =
 inline_for_extraction noextract
 val mod_264: qelem_wide5 -> qelem5
 let mod_264 (t0, t1, t2, t3, t4, t5, t6, t7, t8, t9) =
-  (t0, t1, t2, t3, t4 &. u64 0xffffffffff)
+  (t0, t1, t2, t3, t4 &. mask40)
 
 
 inline_for_extraction noextract
@@ -220,7 +419,7 @@ let div_248 (x0, x1, x2, x3, x4, x5, x6, x7, x8, x9) =
 inline_for_extraction noextract
 val div_2_40_step: x:uint64 -> y:uint64 -> uint64
 let div_2_40_step x y =
-  let y' = (y &. u64 0xffffffffff) <<. 16ul in
+  let y' = (y &. mask40) <<. 16ul in
   let x' = x >>. 40ul in
   let z = y' |. x' in
   z
@@ -268,16 +467,4 @@ val mul_modq5: qelem5 -> qelem5 -> qelem5
 let mul_modq5 (x0, x1, x2, x3, x4) (y0, y1, y2, y3, y4) =
   let (r0, r1, r2, r3, r4, r5, r6, r7, r8, r9) = mul_carry5 (x0, x1, x2, x3, x4) (y0, y1, y2, y3, y4) in
   let (o0, o1, o2, o3, o4) = barrett_reduction5 (r0, r1, r2, r3, r4, r5, r6, r7, r8, r9) in
-  (o0, o1, o2, o3, o4)
-
-
-inline_for_extraction noextract
-val add_modq5: x:qelem5 -> y:qelem5 -> z:qelem5
-let add_modq5 (x0, x1, x2, x3, x4) (y0, y1, y2, y3, y4) =
-  let (carry, x0) = carry56 (x0 +. y0) in
-  let (carry, x1) = carry56 (x1 +. y1 +. carry) in
-  let (carry, x2) = carry56 (x2 +. y2 +. carry) in
-  let (carry, x3) = carry56 (x3 +. y3 +. carry) in
-  let x4 = x4 +. y4 +. carry in
-  let (o0, o1, o2, o3, o4) = subm_conditional (x0, x1, x2, x3, x4) in
   (o0, o1, o2, o3, o4)
